---
title: "notation"
author: "kang wen wei"
date: "2018/6/29"
output: html_document
---

### $y_i=\vec{w}\vec{\mu}+b$

### $\vec{w}為平面參數，\vec{\mu}為\vec{x}的向量$

$$
\begin{equation}
\begin{aligned}
&\Rightarrow
\left\{
\begin{array}{r@{\;=\;}l}
&\vec{w}\bullet\vec{x_+}+b\geq1\\
&\vec{w}\bullet\vec{x_−}+b\leq-1
\end{array}
\right.,
\mbox{such that }y_i=
\left\{
\begin{array}{r@{\;=\;}l}
+1 & ,\mbox{for + examples}\\
-1 & ,\mbox{for − examples}
\end{array}
\right.\\
&\Rightarrow\left\{
\begin{array}{r@{\;=\;}l}
y_i(\vec{w}\vec{x_i}+b)\geq1\\
y_i(\vec{w}\vec{x_i}+b)\geq1
\end{array}
\right.
\Rightarrow y_i(\vec{w}\vec{x_i}+b)-1\geq0\\
&\Rightarrow y_i(\vec{w}\vec{x_i}+b)-1=0
\end{aligned}
\end{equation}
$$

### $\vec{u}=(3,4)$

### $\frac{\vec{u}}{||\vec{u}||}=(\frac{3}{5},\frac{4}{5})$
 
### $x_1=(4,2)$

### $x_2=(8,4)$

### $(x_2-x_1)\bullet\frac{\vec{u}}{||\vec{u}||}=(4,2)\bullet(\frac{3}{5},\frac{4}{5})=4$

### $x_+$

### $x_-$

### $\vec{w}$

$$
\begin{align}
\mbox{width}&=(\vec{x_+}-\vec{x_-})\bullet\frac{\vec{w}}{||\vec{w}||}\\
&=\frac{\vec{x_+}\vec{w}-\vec{x-}\vec{w}}{||\vec{w}||}\\
&=\frac{(1-b)-(-1-b)}{||\vec{w}||}\\
&=\frac{2}{||\vec{w}||}
\end{align}
$$

### $Maximum\;\frac{2}{||\vec{w}||}$

### $y_i(\vec{w}\vec{x_i}+b)-1=0$

### $Condition:$

### $\Rightarrow$

$$
Max\frac{2}{||\vec{w}||}\Rightarrow
Max\frac{1}{||\vec{w}||}\Rightarrow
Min||\vec{w}||\Rightarrow
Min\frac{1}{2}||\vec{w}||^2
$$

### $Min\;\frac{1}{2}||\vec{w}||^2$

### $y=x^2 \Rightarrow \frac{dy}{dx}=2x=0$

### $x=0 \Rightarrow y=0$

### $O:f(x,y)$

### $C:g(x,y)$

$$
L(x,y,\lambda) = f(x,y)-\lambda g(x,y)\\
\begin{equation}
\begin{aligned}
&\left\{
\begin{array}{r@{\;=\;}l}
&\frac{\partial{f}}{\partial{x}}=\lambda\frac{\partial{g}}{\partial{x}}\\
&\frac{\partial{f}}{\partial{y}}=\lambda\frac{\partial{g}}{\partial{y}}\\
&g=0
\end{array}
\right.\;\Rightarrow
x,y,\lambda
\end{aligned}
\end{equation}
$$

$$
\begin{align}
&\sum\lambda_i-\frac{1}{2}\sum_i\sum_j\lambda_i\lambda_jy_iy_j\vec{x_i}\vec{x_j}\;,\lambda_i\geq0\\
\Rightarrow&\sum\lambda_i-\frac{1}{2}\sum_i\sum_j\lambda_i\lambda_jy_iy_jK(\vec{x_i},\vec{x_j})\;,\lambda_i\geq0
\end{align}
$$

### $Linear:K(x_i,x_j)=x_i^Tx_j$

### $Polynomial:K(x_i,x_j)=(\gamma x_i^Tx_j + c)^d , d > 1$

### $Radial\;basis\;function:K(x_i,x_j)=exp(-\gamma ||x_i-x_j||^2), \gamma > 0$

### $K(x_i,x_j) = exp(-\frac{||x_i-x_j||^2}{2\sigma^2})$

### $\phi^T(x_i) \bullet \phi(x_j)$ 

### $\because ||x_i-x_j||^2=x_i^Tx_i+x_j^Tx_j-2x_i^Tx_j$

### $\therefore K(x_i,x_j)=exp(-\frac{x_i^Tx_i}{2\sigma^2})\bullet exp(-\frac{x_j^Tx_j}{2\sigma^2})\bullet exp(\frac{x_i^Tx_j}{\sigma^2})$

### $e^x =1+x+\frac{x^2}{2!}+\frac{x^3}{3!}+...+\frac{x^n}{n!}=\sum_{n=0}^{\infty}\frac{x^n}{n!}$

$$
\begin{align}
exp(\frac{x_i^Tx_j}{\sigma^2})
&= \sum_{n=0}^{\infty}\frac{1}{n!}\bullet \frac{(x_i^Tx_j)^n}{\sigma^{2n}}\\
&= \sum_{n=0}^{\infty}\frac{1}{\sqrt{n!}}\bullet \frac{(x_i^T)^n}{\sigma^n}\bullet \frac{1}{\sqrt{n!}}\bullet \frac{(x_j^T)^n}{\sigma^n} \\
&= \varphi^T(x_i)\bullet \varphi(x_j)
\end{align}
$$

$$
\begin{align}
K(x_i,x_j)&=exp(-\frac{x_i^Tx_i}{2\sigma^2})\bullet exp(-\frac{x_j^Tx_j}{2\sigma^2})\bullet exp(\frac{x_i^Tx_j}{\sigma^2})\\
&= exp(-\frac{x_i^Tx_i}{2\sigma^2})\bullet exp(\frac{x_i^Tx_j}{\sigma^2})\bullet exp(-\frac{x_j^Tx_j}{2\sigma^2})\\
&= exp(-\frac{x_i^Tx_i}{2\sigma^2})\bullet \varphi^T(x_i)\bullet \varphi(x_j)\bullet exp(-\frac{x_j^Tx_j}{2\sigma^2})\\
&=\phi^T(x_i)\bullet \phi(x_j)\\
其中&: \phi^T(x_i)=exp(-\frac{x_i^Tx_i}{2\sigma^2})\bullet \varphi^T(x_i)\\
&\varphi^T(x)=\sum_{n=0}^{\infty}\frac{1}{\sqrt{n!}}\bullet \frac{(x^T)^n}{\sigma^n}
\end{align}
$$





